fixed the spec, proof of OK loop case, refactored lemma statements

src/C_strtoimax/Spec.v
@@ -44,13 +44,13 @@ Definition zero_char := (Int.repr 48).
 (* Representing negative and positive int using signedness *)
 Definition int_to_int64 (i : int) := Int64.repr (Int.signed i).
 
-Definition Sign s :=
+Definition sign_to_int s :=
   match s with
   | Signed => (Int.repr (-1))
   | Unsigned => Int.repr 1
   end.
 
-Definition sign i :=
+Definition char_to_sign i :=
   if (i == minus_char)%int then Signed else Unsigned.
 
 Definition mult_sign s value :=
@@ -95,22 +95,19 @@ Definition digit_to_num s i v :=
     { return_type : asn_strtox_result_e ;
       value : option int64 ;
       str_pointer : option addr ;
-      memory : option mem ; 
+      memory : option mem ;
+      sign : signedness ;
       }.
-  
-
-  Fixpoint asn_strtoimax_lim_loop (str fin intp : addr) (value : int64)
+    
+  Fixpoint asn_strtoimax_lim_loop' (str fin intp : addr) (value : int64)
            (s: signedness) (last_digit : int64)
            (dist : nat) (m'' : mem) {struct dist} : option asn_strtoimax_lim_result := 
     match dist with
-    | O => match (Mem.storev Mptr m'' (vptr fin) (vptr str)) with
-          | Some m' => 
-            Some {| return_type := ASN_STRTOX_OK;
-                    value := Some (mult_sign s value);
-                    str_pointer := Some str;
-                    memory := Some m'' |}
-          | None => None
-          end
+    | O => Some {| return_type := ASN_STRTOX_OK;
+                  value := Some value;
+                  str_pointer := Some str;
+                  memory := Some m'';
+                  sign := s; |}
     | S n => match load_addr Mint8signed m'' str with
             | Some (Vint i) =>
               if is_digit i
@@ -118,17 +115,21 @@ Definition digit_to_num s i v :=
               then let d := int_to_int64 (i - zero_char)%int in
                    (* int d = *str - '0' *)
                    if value < upper_boundary
-                   then asn_strtoimax_lim_loop (str++) fin intp
+                   then asn_strtoimax_lim_loop' (str++) fin intp
                         (value * (Int64.repr 10) + d) s last_digit n m
                         (* value = value * 10 + d; next iteration *)
-                   else if (value == upper_boundary) && (d <= last_digit_max)
+                   else if (value == upper_boundary) && (d <= last_digit)
                         (* firstly check if str < *end, and if so, return *)
                         then let value' := digit_to_num s i value in
-                             let s' := match s with | Signed => Unsigned | _ => Unsigned end in
+                             let s' := match s with 
+                                       | Signed => Unsigned 
+                                       | _ => Unsigned 
+                                       end in
                              match (Mem.loadv Mptr m'' (vptr fin)) with
                              | Some (Vptr b fin') =>
                                match addr_lt m'' (str++) (b, fin') with
-                               | Some true => match (load_addr Mint8signed m'' (str++)) with
+                               | Some true => match (load_addr Mint8signed m'' 
+                                                              (str++)) with
                                           | Some (Vint i') =>
                                             if is_digit i'
                                             then Some {|
@@ -137,8 +138,9 @@ Definition digit_to_num s i v :=
                                                      str_pointer := None;
                                                      memory := (Mem.storev Mptr m'' 
                                                                            (vptr (b, fin')) 
-                                                                           (vptr (str++))) |}
-                                            else match Mem.storev Mptr m'' (vptr (b, fin'))
+                                                                           (vptr (str++)));
+                                                     sign := s'; |}
+                                            else match Mem.storev Mptr m'' (vptr (b, fin')) 
                                                                               (vptr (str++)) with
                                                  | Some m' => 
                                                    Some {| 
@@ -146,48 +148,70 @@ Definition digit_to_num s i v :=
                                                        value := Some (mult_sign s' value');
                                                        str_pointer := Some str;
                                                        memory := Mem.storev Mint64 m' (vptr intp)
-                                                                  (Vlong (mult_sign s' value')) |}
+                                                              (Vlong (mult_sign s' value'));
+                                                       sign := s'; |}
+                               
                                                  | _ => None
                                                  end
                                           | _ => None
                                           end
+                               | Some false => Some {|
+                                                  return_type := ASN_STRTOX_OK;
+                                                  value := Some (mult_sign s' value');
+                                                  str_pointer := Some (str++);
+                                                  memory := Some m'';
+                                                  sign := s' |}
                                | _ => None
                                end
                              | _ => None
                              end
                         else match (Mem.storev Mptr m'' (vptr fin) (vptr str)) with
                              | Some m' => 
-                               Some {| return_type := ASN_STRTOX_ERROR_RANGE;
-                                       value := None;
-                                       str_pointer := None;
-                                       memory := Some m' |}
+                               Some {|
+                                   return_type := ASN_STRTOX_ERROR_RANGE;
+                                   value := None;
+                                   str_pointer := None;
+                                   memory := Some m';
+                                   sign := s; |}
                              | None => None
                              end                          
               else match (Mem.storev Mptr m'' (vptr fin) (vptr str)) with
                    | Some m' => Some {| return_type := ASN_STRTOX_EXTRA_DATA;
-                                        value := Some (mult_sign s value);
-                                        str_pointer := Some str;
+                                       value := Some (mult_sign s value);
+                                       str_pointer := Some str;
                                        memory := Mem.storev Mint64 m' (vptr intp) 
-                                                            (Vlong (mult_sign s value)) |}
+                                                            (Vlong (mult_sign s value));
+                                       sign := s; |}
                    | None => None
                    end
             | _ => None                
             end
     end.
 
-Definition store_result s fin intp res :=
+  Definition asn_strtoimax_lim_loop (str fin intp : addr) (value : int64) 
+             (s: signedness) (last_digit : int64) 
+             (dist : option nat) (m : mem) : option asn_strtoimax_lim_result := 
+    match dist with
+    | Some d => 
+      asn_strtoimax_lim_loop' str fin intp value s last_digit d m
+    | None => None
+    end.
+
+Definition store_result fin intp res :=
   match res with
   | Some {| return_type := ASN_STRTOX_OK;
             value := Some val;
             str_pointer := Some str;
-            memory := Some m'; |} =>
+            memory := Some m';
+            sign := s; |} =>
     match (Mem.storev Mptr m' (vptr fin) (vptr str)) with
     | Some m'' =>
       Some {| return_type := ASN_STRTOX_OK;
               value := Some (mult_sign s val);
               str_pointer := Some str;
               memory := Mem.storev Mint64 m'' (vptr intp)
-                                   (Vlong (mult_sign s val)) |}
+                                   (Vlong (mult_sign s val));
+              sign := s; |}
     | None => None
     end
   | _ => res
@@ -198,32 +222,42 @@ Definition asn_strtoimax_lim (str fin intp : addr) : option asn_strtoimax_lim_re
   | Some (Vptr b ofs) =>
     match addr_ge m str (b, ofs) with (* compare str and *fin *)
     | Some true => Some {| return_type := ASN_STRTOX_ERROR_INVAL;
-                           value := None;
-                           str_pointer := None;
-                           memory := Some m; |}
-    | Some false => let dist := distance str (b,ofs) in
-                   match load_addr Mint8signed m str with
-                   | Some (Vint i) =>
-                     if (i == minus_char)%int || (i == plus_char)%int
-                     then match addr_ge m (str++) (b,ofs) with
-                          | Some true =>
-                            Some {| return_type := ASN_STRTOX_EXPECT_MORE;
-                                    value := None;
-                                    str_pointer := Some str;
-                                    memory := (Mem.storev Mptr m
-                                                          (vptr fin)
-                                                          (vptr (str++))); |}
-
-                          | Some false => store_result (sign i) fin intp
-                                           (asn_strtoimax_lim_loop
-                                           (str++) fin intp 0 (sign i)
-                                           (max_sign (sign i)) (dist - 1)%nat m)
-                          | None => None
-                          end
-                     else store_result Unsigned fin intp
-                            (asn_strtoimax_lim_loop str fin intp 0
-                                Unsigned last_digit_max dist m)
-                   | _ => None (* fail of memory load on str: wrong type or not enough permission *)
+                          value := None;
+                          str_pointer := None;
+                          memory := Some m;
+                          sign := Unsigned; |}
+    | Some false => match distance m str (b,ofs) with 
+                   | Some dist => 
+                     match load_addr Mint8signed m str with 
+                     | Some (Vint i) => 
+                       if (i == minus_char)%int || (i == plus_char)%int 
+                       then match addr_ge m (str++) (b,ofs) with 
+                            | Some true => 
+                              Some {| return_type := ASN_STRTOX_EXPECT_MORE; 
+                                      value := None; 
+                                      str_pointer := Some str; 
+                                      memory := (Mem.storev Mptr m 
+                                                            (vptr fin) 
+                                                            (vptr (str++)));
+                                      sign := (char_to_sign i) |} 
+                            | Some false => store_result fin intp 
+                                                        (asn_strtoimax_lim_loop 
+                                                           (str++) fin intp 0
+                                                           (char_to_sign i) 
+                                                           (max_sign (char_to_sign i))
+                                                           (Some (dist - 1)%nat) m) 
+                            | None => None 
+                            end 
+                       else store_result fin intp 
+                                         (asn_strtoimax_lim_loop
+                                            str fin intp 0
+                                            Unsigned
+                                            last_digit_max
+                                            (Some dist) m) 
+                     | _ => None (* fail of memory load on str:
+ wrong type or not enough permission *) 
+                     end
+                   | None => None
                    end
     | None => None (* error in pointer comparison *)
     end
