src/C_strtoimax/Proof.v
@@ -10,26 +10,28 @@ Local Open Scope Int64Scope.
 
 (* ASN_STRTOX_ERROR_INVAL: str >= *end *)
 Lemma asn_strtoimax_lim_ASN_STRTOX_ERROR_INVAL_correct :
-  forall m ge e le str_b str_ofs fin_b fin_ofs intp_b intp_ofs m' p val,
+  forall m ge e le b str_ofs fin_ofs intp_ofs m' p s' val,
     
-    le ! _str = Some (Vptr str_b str_ofs)  ->
-    le ! _end = Some (Vptr fin_b fin_ofs) ->
-    le ! _intp = Some (Vptr intp_b intp_ofs)  ->
+    le ! _str = Some (Vptr b str_ofs)  ->
+    le ! _end = Some (Vptr b fin_ofs) ->
+    le ! _intp = Some (Vptr b intp_ofs)  ->
     le ! _upper_boundary = Some (Vlong upper_boundary) ->
     le ! _sign = Some (Vint (Int.repr 1)) ->
 
-    asn_strtoimax_lim m (str_b, str_ofs) (fin_b,fin_ofs) (intp_b,intp_ofs) =
+    asn_strtoimax_lim m (b, str_ofs) (b, fin_ofs) (b, intp_ofs) =
     Some {| return_type := ASN_STRTOX_ERROR_INVAL;
             value := val;
-            str_pointer := p;
-        memory := Some m' |} ->
+            str_pointer := p; 
+            memory := Some m';
+            sign := s';
+         |} ->
     
     exists (t : trace) (le' : temp_env),
       exec_stmt ge e le m (fn_body f_asn_strtoimax_lim) t le' m'
-                (Out_return (Some (Vint (asn_strtox_result_e_to_int ASN_STRTOX_ERROR_INVAL), tint))).
+                (Out_return (Some (Vint (asn_strtox_result_e_to_int 
+                                           ASN_STRTOX_ERROR_INVAL), tint))).
 Proof.
   intros until val; intros Str End Intp UB Sign Spec.
-  simpl in Spec.                       
   unfold asn_strtoimax_lim in Spec.
   assert (forall dist str fin inp value s last_digit,
              asn_strtoimax_lim_loop m str fin inp value s last_digit dist m
@@ -37,12 +39,16 @@ Proof.
                     return_type := ASN_STRTOX_ERROR_INVAL;
                     value := val;
                     str_pointer := p;
-                    memory := Some m' |}) as Loop.
-    { induction dist; intros; simpl.
-      + break_match;
-        congruence.
-      + repeat break_match;
-          congruence.
+                    memory := Some m';
+                    sign := s'; |}) as Loop.
+    { destruct dist as [dist|]. 
+      - induction dist; intros; simpl. 
+        + break_match; 
+            congruence. 
+        + repeat break_match;
+          unfold asn_strtoimax_lim_loop in IHdist;
+            congruence.
+      - discriminate.
     } 
     repeat break_match; unfold store_result in *;
       repeat break_match; try congruence.
@@ -75,47 +81,55 @@ Proof.
   eapply exec_Sreturn_some.
   econstructor.
   discriminate.
-Admitted.
+Qed.
+
 
 (* SN_STRTOX_EXPECT_MORE: reading + or - and reaching *end *)
 (* ASN_STRTOX_EXPECT_MORE: reading + or - and reaching *end *)
 Lemma asn_strtoimax_lim_ASN_STRTOX_EXPECT_MORE_correct :
 
-  forall m ge e le str_b str_ofs fin_b fin_ofs intp_b intp_ofs m' p val,
+  forall m ge e le b str_ofs fin_ofs intp_ofs m' p s' val,
     
-    le!_str = Some (Vptr str_b str_ofs)  ->
-    le!_end = Some (Vptr fin_b fin_ofs) ->
-    le!_intp = Some (Vptr intp_b intp_ofs)  ->
+    le ! _str = Some (Vptr b str_ofs)  ->
+    le ! _end = Some (Vptr b fin_ofs) ->
+    le ! _intp = Some (Vptr b intp_ofs)  ->
     le ! _upper_boundary = Some (Vlong upper_boundary) ->
     le ! _sign = Some (Vint (Int.repr 1)) ->
 
-    asn_strtoimax_lim m (str_b, str_ofs) (fin_b,fin_ofs) (intp_b,intp_ofs) =
+    asn_strtoimax_lim m (b, str_ofs) (b, fin_ofs) (b, intp_ofs) =
     Some
       {|
         return_type := ASN_STRTOX_EXPECT_MORE;
         value := val;
         str_pointer := p;
-        memory := Some m' |} ->
+        memory := Some m';
+        sign := s';
+      |} ->
     
     exists (t : trace) (le' : temp_env),
       exec_stmt ge e le m (fn_body f_asn_strtoimax_lim) t le' m'
-                (Out_return (Some (Vint (asn_strtox_result_e_to_int ASN_STRTOX_EXPECT_MORE), tint))).
+                (Out_return (Some (Vint (asn_strtox_result_e_to_int 
+                                           ASN_STRTOX_EXPECT_MORE), tint))).
 Proof.
   replace (asn_strtox_result_e_to_int ASN_STRTOX_EXPECT_MORE)
     with (Int.repr (-1)) by reflexivity.
   intros until val; intros Str End Intp UB Sign Spec.
   simpl in Spec.    
-  assert (forall dist str fin intp v s last_digit m',
+  assert (forall dist str fin intp v s last_digit m', 
              asn_strtoimax_lim_loop m str fin intp v s last_digit dist m <>
              Some {| return_type := ASN_STRTOX_EXPECT_MORE;
                      value := val;
-                     str_pointer := p;
-                  memory := Some m' |}) as Loop.
-    { induction dist; intros; simpl.
-      + break_match; congruence.
-      + repeat break_match.
-        repeat break_if.
-        all: try congruence; eapply IHdist. }
+                     str_pointer := p; 
+                     memory := Some m';
+                     sign := s';|}) as Loop.
+    { destruct dist as [dist|].
+      - induction dist; intros; simpl. 
+        + try break_match; congruence. 
+        + repeat break_match. 
+          repeat break_if. 
+          all: try congruence; eapply IHdist.
+      - discriminate.
+    }
    unfold asn_strtoimax_lim in Spec.  
     repeat break_match;
       unfold store_result in *;
@@ -188,69 +202,320 @@ Proof.
       Tactics.forward.
       eapply ptr_ge_to_sem_cmp_true; eassumption.
       all: Tactics.forward; try discriminate.
-  - pose proof (Loop (distance (str_b, str_ofs) (b, i) - 1)%nat ((str_b, str_ofs) ++)
-                     (fin_b, fin_ofs) (intp_b, intp_ofs) 0 (sign i0)
-                     (max_sign (sign i0)) m'). admit. (* congruence. *)
-  - pose proof (Loop (distance (str_b, str_ofs) (b, i))%nat ((str_b, str_ofs))
-                     (fin_b, fin_ofs) (intp_b, intp_ofs) 0  Unsigned
-                     last_digit_max  m'). admit. (* congruence. *)
-Admitted.
+  - pose proof (Loop (Some (n - 1)%nat) ((b, str_ofs) ++) 
+                     (b, fin_ofs) (b, intp_ofs) 0 (char_to_sign i0) 
+                     (max_sign (char_to_sign i0)) m'). 
+      congruence.
+  - pose proof (Loop (Some n) ((b, str_ofs)) 
+                     (b, fin_ofs) (b, intp_ofs) 0 Unsigned 
+                     last_digit_max m'). congruence.
+Qed.
 
 (* Loop correctness cases *)
 (* ASN_STRTOX_OK: conversion successfull *)
 Lemma asn_strtoimax_lim_loop_ASN_STRTOX_OK_correct :
   forall m ge e dist b ofs le strp_b strp_ofs str_b str_ofs fin_b fin_ofs intp_b intp_ofs
-         inp_value  m' val s,
+         inp_value  m' val s' s,
     
     le!_str = Some (Vptr str_b str_ofs)  ->
     le!_end = Some (Vptr fin_b fin_ofs) ->
     le!_intp = Some (Vptr intp_b intp_ofs) ->
     le!_value = Some (Vlong inp_value) ->
     le ! _upper_boundary = Some (Vlong upper_boundary) ->
-    le ! _sign = Some (Vint (Sign s)) ->
+    le ! _sign = Some (Vint (sign_to_int s)) ->
+    le ! _last_digit_max = Some (Vlong (max_sign s)) ->
 
     load_addr Mptr m (fin_b, fin_ofs) = Some (Vptr b ofs) ->
 
-    (distance (str_b, str_ofs) (b,ofs)) = dist ->
+    (distance m (str_b, str_ofs) (b,ofs)) = Some dist ->
 
     asn_strtoimax_lim_loop m (str_b, str_ofs) (fin_b, fin_ofs)
-                           (intp_b, intp_ofs) inp_value s (max_sign s) dist m =
+                           (intp_b, intp_ofs) inp_value s (max_sign s) (Some dist) m =
     Some {| return_type := ASN_STRTOX_OK;
             value := Some val;
             str_pointer := Some (strp_b, strp_ofs);
-            memory := Some m'; 
+            memory := Some m';
+            sign := s';
          |}  ->
 
     exists t le', exec_stmt ge e le m f_asn_strtoimax_lim_loop t le' m Out_normal
              /\ le'! _end = Some (Vptr fin_b fin_ofs)
              /\ le'! _str = Some (Vptr strp_b strp_ofs)
-             /\ le'! _sign = Some (Vint (Sign s))
+             /\ le'! _sign = Some (Vint (sign_to_int s'))
              /\ le'! _intp = Some (Vptr intp_b intp_ofs)
              /\ le'! _value = Some (Vlong val)
              /\ m' = m.
+Proof.
+  induction dist; intros until s;
+  intros Str End Intp Value UB Sign LastD Load Dist Spec;
+  simpl in Spec.
+  - all: try break_match; try congruence.
+    inversion Spec.
+    rewrite <- H3.
+    (* break from the loop, follows from distance *)
+    repeat eexists.
+    eapply exec_Sloop_stop1.
+    eapply exec_Sseq_2.
+    forward.
+    simpl.
+    enough (sem_cmp Clt (Vptr str_b str_ofs) (tptr tschar) (Vptr b ofs) (tptr tschar) m
+            = Some Vfalse) by eassumption.
+    admit.
+    forward.
+    all: repeat (env_assumption || econstructor
+                 || discriminate).
+    rewrite <- H1.
+    rewrite <- H2.
+    assumption.
+    rewrite <- H4.
+    eassumption.
+    rewrite <- H0.
+    eassumption.
+  - repeat break_match;
+    unfold store_result in *;
+      repeat break_match; try congruence.
+    + (* Case   Heqb0 : is_digit i = true
+         Heqb1 : (inp_value < upper_boundary) = true *)
+      remember 
+         (PTree.set _str
+       (Vptr str_b
+             (str_ofs + Ptrofs.repr (sizeof ge tschar)
+                        * ptrofs_of_int Signed (Int.repr 1))%ptrofs)
+       (PTree.set _value
+          (Vlong
+             (inp_value * cast_int_long Signed (Int.repr 10) +
+              cast_int_long Signed (i - Int.repr 48)%int))
+          (PTree.set _d (Vint (i - Int.repr 48)%int)
+             (PTree.set _t'6 (Vint i)
+                (PTree.set _t'2 Vtrue
+                   (PTree.set _t'8 (Vint i)
+                    (PTree.set _t'7 (Vint i) (PTree.set _t'9 (Vptr b ofs) le))))))))
+        as le''.
+      pose proof (IHdist b ofs le'' strp_b strp_ofs str_b (str_ofs + 1)%ptrofs
+                         fin_b fin_ofs intp_b intp_ofs
+                         (digit_to_num Unsigned i inp_value) m' val s' s) as IH.
+      clear IHdist.
+      repeat rewrite set_env_eq_ptree_set in Heqle''.
+      destruct IH as [t IH]; subst;
+        try (repeat env_assumption || reflexivity).
+      { eapply dist_succ. eassumption.
+        unfold distance in *.
+        admit.
+      }
+      destruct IH as [le' IH]. 
+      repeat rewrite set_env_eq_ptree_set in *.
+      repeat eexists.
+      eapply exec_Sloop_loop.
+      instantiate (1 := Out_normal).
+      econstructor. (* Wrong local env instantiated  by repeat econstructor ??? *)
+      econstructor.
+      econstructor.
+      repeat econstructor; try env_assumption.
+      repeat econstructor; try env_assumption.
+      try eassumption.
+      econstructor.
+      assert (sem_cmp Clt (Vptr str_b str_ofs) (tptr tschar)
+                      (Vptr b ofs) (tptr tschar) m = Some Vtrue).
+      { admit. }
+      eassumption.
+      repeat econstructor.
+      replace (negb (1 == 0)%int) with true by (auto with ints).
+      econstructor.
+      econstructor.
+      repeat econstructor; try env_assumption; try eassumption.
+      forward.
+      simpl.
+      unfold is_digit in Heqb0.
+      destruct_andb_hyp.
+      apply sem_Cle_Cge.
+      apply int_le_sem_Cle.
+      assumption.
+      forward.
+      replace (negb (1 == 0)%int) with true by (auto with ints).
+      econstructor.
+      econstructor.
+      repeat econstructor; try env_assumption; try eassumption.
+      forward.
+      forward.
+      simpl.
+      unfold is_digit in Heqb0.
+      destruct_andb_hyp.
+      rewrite H0.
+      reflexivity.
+      forward.
+      simpl.
+      rewrite Heqb1.
+      econstructor.
+      replace (negb (1 == 0)%int) with true by (auto with ints).
+      forward.
+      econstructor.
+      forward.
+      fold f_asn_strtoimax_lim_loop.
+      eapply IH.
+      all: break_and; eassumption.
+    + (* Case (inp_value == upper_boundary) 
+           && (int_to_int64 (i - zero_char)%int <= last_digit_max) = true 
+         addr_lt m (str_b, (str_ofs + 1)%ptrofs) (b0, i0) = Some false
+         Signed 
+       *) (* go through one loop and break *)
+      unfold max_sign in *.
+      unfold is_digit in *.
+      repeat destruct_andb_hyp.
+      repeat eexists.
+      eapply exec_Sloop_stop1.
+      instantiate (1 := Out_break).
+      econstructor. (* Wrong local env instantiated  by repeat econstructor ??? *)
+      econstructor.
+      econstructor.
+      repeat econstructor; try env_assumption.
+      repeat econstructor; try env_assumption.
+      try eassumption.
+      econstructor.
+      assert (sem_cmp Clt (Vptr str_b str_ofs) (tptr tschar)
+                      (Vptr b0 i0) (tptr tschar) m = Some Vtrue).
+      { admit. }
+      eassumption.
+      repeat econstructor.
+      replace (negb (1 == 0)%int) with true by (auto with ints).
+      econstructor.
+      econstructor.
+      repeat econstructor; try env_assumption; try eassumption.
+      forward.
+      simpl.
+      apply sem_Cle_Cge.
+      apply int_le_sem_Cle.
+      assumption.
+      forward.
+      replace (negb (1 == 0)%int) with true by (auto with ints).
+      econstructor.
+      econstructor.
+      repeat econstructor; try env_assumption; try eassumption.
+      forward.
+      forward.
+      simpl.
+      bool_rewrite.
+      reflexivity.
+      forward.
+      simpl.
+      bool_rewrite.
+      econstructor.
+      replace (negb (1 == 0)%int) with true by (auto with ints).
+      forward.
+      simpl.
+      repeat destruct_andb_hyp.
+      bool_rewrite.
+      econstructor.
+      forward.
+      simpl.
+      unfold int_to_int64 in *.
+      unfold zero_char in *.
+      bool_rewrite.
+      forward.
+      replace (negb (1 == 0)%int) with true by (auto with ints).
+      forward.
+      simpl.
+      enough (sem_cmp Clt (Vptr str_b (str_ofs + 1)%ptrofs)
+                      (tptr tschar) (Vptr b0 i0) (tptr tschar) m = Some Vfalse)
+        by eassumption.
+      admit.
+      forward.
+       all: repeat (env_assumption || econstructor
+                    || discriminate).
+       all: inversion Spec;
+       reflexivity.
+      + (* Case (inp_value == upper_boundary) 
+           && (int_to_int64 (i - zero_char)%int <= last_digit_max) = true 
+         addr_lt m (str_b, (str_ofs + 1)%ptrofs) (b0, i0) = Some false
+         Unsigned *)
+        (* go through one loop and break *)
+      unfold max_sign in *.
+      unfold is_digit in *.
+      repeat destruct_andb_hyp.
+      repeat eexists.
+      eapply exec_Sloop_stop1.
+      instantiate (1 := Out_break).
+      econstructor. 
+      econstructor.
+      econstructor.
+      repeat econstructor; try env_assumption.
+      repeat econstructor; try env_assumption.
+      try eassumption.
+      econstructor.
+      assert (sem_cmp Clt (Vptr str_b str_ofs) (tptr tschar)
+                      (Vptr b0 i0) (tptr tschar) m = Some Vtrue).
+      { admit. }
+      eassumption.
+      repeat econstructor.
+      replace (negb (1 == 0)%int) with true by (auto with ints).
+      econstructor.
+      econstructor.
+      repeat econstructor; try env_assumption; try eassumption.
+      forward.
+      simpl.
+      apply sem_Cle_Cge.
+      apply int_le_sem_Cle.
+      assumption.
+      forward.
+      replace (negb (1 == 0)%int) with true by (auto with ints).
+      econstructor.
+      econstructor.
+      repeat econstructor; try env_assumption; try eassumption.
+      forward.
+      forward.
+      simpl.
+      bool_rewrite.
+      reflexivity.
+      forward.
+      simpl.
+      bool_rewrite.
+      econstructor.
+      replace (negb (1 == 0)%int) with true by (auto with ints).
+      forward.
+      simpl.
+      repeat destruct_andb_hyp.
+      bool_rewrite.
+      econstructor.
+      forward.
+      simpl.
+      unfold int_to_int64 in *.
+      unfold zero_char in *.
+      bool_rewrite.
+      forward.
+      replace (negb (1 == 0)%int) with true by (auto with ints).
+      forward.
+      simpl.
+      enough (sem_cmp Clt (Vptr str_b (str_ofs + 1)%ptrofs)
+                      (tptr tschar) (Vptr b0 i0) (tptr tschar) m = Some Vfalse)
+        by eassumption.
+      admit.
+      forward.
+      all: inversion Spec;
+        repeat (env_assumption || econstructor
+                    || discriminate).
 Admitted.
 
  Lemma asn_strtoimax_lim_loop_ASN_STRTOX_ERROR_RANGE_correct :
    forall m ge e dist b ofs le str_b str_ofs fin_b fin_ofs
-          intp_b intp_ofs inp_value  m' p val s,
+          intp_b intp_ofs inp_value  m' p val s' s,
     
     le!_str = Some (Vptr str_b str_ofs)  ->
     le!_end = Some (Vptr fin_b fin_ofs) ->
     le!_intp = Some (Vptr intp_b intp_ofs)  ->
     le!_value = Some (Vlong inp_value) ->
     le ! _upper_boundary = Some (Vlong upper_boundary) ->
-    le ! _sign = Some (Vint (Sign s)) ->
+    le ! _sign = Some (Vint (sign_to_int s)) ->
 
     load_addr Mptr m (fin_b, fin_ofs) = Some (Vptr b ofs) ->
 
-    (distance (str_b, str_ofs) (b,ofs)) = dist ->
+    (distance m (str_b, str_ofs) (b,ofs)) = dist ->
 
     asn_strtoimax_lim_loop m (str_b, str_ofs) (fin_b, fin_ofs)
                            (intp_b, intp_ofs) inp_value s (max_sign s) dist m =
     Some {| return_type := ASN_STRTOX_ERROR_RANGE;
             value := val;
             str_pointer := p;
-            memory := Some m'; 
+            memory := Some m';
+            sign := s';
            |}  ->
 
     exists t le', exec_stmt ge e le m f_asn_strtoimax_lim_loop t le' m' (Out_return (Some (Vint (asn_strtox_result_e_to_int ASN_STRTOX_ERROR_RANGE), tint))).         
@@ -259,25 +524,28 @@ Admitted.
 
 Lemma asn_strtoimax_lim_loop_ASN_STRTOX_EXTRA_DATA_correct :
   forall m ge e dist b ofs le str_b str_ofs fin_b 
-    fin_ofs intp_b intp_ofs inp_value  m' p val s,
+    fin_ofs intp_b intp_ofs inp_value  m' p val s' s,
     
     le ! _str = Some (Vptr str_b str_ofs)  ->
     le ! _end = Some (Vptr fin_b fin_ofs) ->
     le ! _intp = Some (Vptr intp_b intp_ofs)  ->
     le ! _value = Some (Vlong inp_value) ->
     le ! _upper_boundary = Some (Vlong upper_boundary) ->
-    le ! _sign = Some (Vint (Sign s)) ->
+    le ! _sign = Some (Vint (sign_to_int s)) ->
     le ! _last_digit_max = Some (Vlong (max_sign s)) ->
                                      
     load_addr Mptr m (fin_b, fin_ofs) = Some (Vptr b ofs) ->
-    (distance (str_b, str_ofs) (b,ofs)) = dist ->
+    (distance m (str_b, str_ofs) (b,ofs)) = Some dist ->
     
     asn_strtoimax_lim_loop m (str_b, str_ofs) (fin_b, fin_ofs) (intp_b, intp_ofs)
-                           inp_value s (max_sign s) dist m =
+                           inp_value s (max_sign s) (Some dist) m =
     Some {| return_type := ASN_STRTOX_EXTRA_DATA;
             value := val;
             str_pointer := p;
-            memory := Some m';|}  ->
+            memory := Some m';
+            sign := s';
+
+         |}  ->
 
     exists t le', exec_stmt ge e le m f_asn_strtoimax_lim_loop t le' m' 
                        (Out_return (Some (Vint (asn_strtox_result_e_to_int 
