src/C_strtoimax/SpecLemmas.v
@@ -3,35 +3,40 @@ Require Import Core.Core.
 Require Import Spec. 
 
 Lemma OK_None_contradiction_1 :
-  forall dist str fin inp value s last_digit m m' val,
+  forall dist str fin inp value s last_digit m m' s' val,
     asn_strtoimax_lim_loop m str fin inp value s last_digit dist m
     <> Some {| return_type := ASN_STRTOX_OK;
-              value := val;
-              str_pointer := None;
-              memory := Some m'
-           |}.
+               value := val;
+               str_pointer := None;
+               memory := Some m';
+               sign := s'; |}.
 Proof.
-  induction dist; intros; simpl.
-    + break_match;
-      congruence.
-    + repeat break_match;
-        try congruence.
-      eapply IHdist.
+  destruct dist as [dist |].
+    - induction dist; intros; simpl.
+      + try congruence.
+      + repeat break_match; 
+          try congruence.
+        unfold asn_strtoimax_lim_loop in IHdist.
+        eapply IHdist.
+    - discriminate.
 Qed.
 
 Proposition OK_None_contradiction_2 :
-  forall dist str fin inp value s last_digit m m' p,
+  forall dist str fin inp value s last_digit m m' s' p,
     asn_strtoimax_lim_loop m str fin inp value s last_digit dist m
     <> Some {| return_type := ASN_STRTOX_OK;
-              value := None;
-              str_pointer := p;
-              memory := Some m'
-           |}.
+               value := None;
+               str_pointer := p;
+               memory := Some m';
+               sign := s'; |}.
 Proof.
-  induction dist; intros; simpl.
-    + break_match;
-      congruence.
-    + repeat break_match;
-        try congruence.
-      eapply IHdist.
+  destruct dist as [dist |].
+    - induction dist; intros; simpl.
+      + try break_match;
+          congruence.
+      + repeat break_match; 
+          try congruence.
+        unfold asn_strtoimax_lim_loop in IHdist.
+        eapply IHdist.
+    - discriminate.
 Qed.
